ViewFunctions.v
@@ -41,6 +41,9 @@ Definition take_left {T : List nat} {n : nat} (b : nat) (v : ViewArray [[T;b+n]]
 Definition take_right {T : List nat} {n : nat} (a : nat) (v : ViewArray [[T;a+n]]) : ViewArray [[T;n]] :=
   fun i => v (idx (a+n) (a + to_nat i) takerightProof).
 
+Definition select_range {T : List nat} {n : nat} (a : nat) (b : nat) (v : ViewArray [[T;b+n]]) : ViewArray [[T;(b-a)]] :=
+  fun i => v (idx (b+n) (a + to_nat i) selectrangeProof).
+
 Definition transpose {T : List nat} {n : nat} {m : nat} (v : ViewArray [[ [[T;m]];n ]]) : ViewArray [[ [[T;n]];m ]] :=
   fun i j => v j i.
 
